\documentclass[12pt]{article}
\usepackage[utf8]{inputenc}
\usepackage[english]{babel}
\usepackage{cite}
\usepackage[]{amsthm} %lets us use \begin{proof}
\usepackage[]{amssymb} %gives us the character \varnothing
\usepackage[ruled,vlined]{algorithm2e}
\usepackage{listings}
\usepackage[utf8]{inputenc}
\usepackage{amsmath}
\usepackage{graphicx}
% One inch margins
\PassOptionsToPackage{margin=0.75in}{geometry}
\title{Modern Optimization Final Exam}
\author{Guanhua Huang}
\date\today

\begin{document}
\maketitle %This command prints the title based on information entered above
\begin{section}{Problem 12}
	\begin{figure}[htp]
		\centering
		\includegraphics[width=12cm]{problem12.png}
	\end{figure}
\subsection{Part a}
\subsection{Part b}
\subsection{Part c}
\end{section}



\begin{section}{Problem 15}
	
	\begin{figure}[htp]
		\centering
		\includegraphics[width=12cm]{problem15.png}
	\end{figure}
	\subsection{Part 1}
	First, let's write the matrix format of the function,

	$$(x_1, x_2) \begin{pmatrix}
	a_1 & a_2\\
	a_2 & a_3 \end{pmatrix}
	\begin{pmatrix}
	x_1\\ 
	x_2
	\end{pmatrix} + (b_1, b_2) \begin{pmatrix}
	x_1\\
	x_2
	\end{pmatrix}$$
	\[= (a_1x_1 + a_2x_2, a_2x_1+a_3x_2) \begin{pmatrix}
	x_1\\
	x_2
	\end{pmatrix} + x_1b_1 + x_2b_2\]
	\[(a_1x_1 + a_2x_2)x_1 + (a_2x_1 + a_3x_2)x_2 + x_1b_1 + x_2b_2\]
	\[=a_1x_1^2 + 2a_2x_1x_2 + a_3x_2^2 + b_1x_1 + b_2x_2\]
	\[=-12x_2 + 4x_1^2 + 4x_2^2-4x_1x_2\]	

	By comparing parameters, we got the following, 
	\[b_2 = -12, b_1 = 0, a_2 = -2, a_1 =a_3 = 4\]
	\[A = \begin{pmatrix}
	4 & -2\\
	-2 & 4 
	\end{pmatrix}, b = \begin{pmatrix}
	0\\
	-12
	\end{pmatrix}\]
	
	Based on A-conjugate definition (on page 120), $\langle d_1, Ad_2 \rangle = 0, \;\; d_1 = (1,0)^T$, then, let's write out the problem as the following: 
	
	$$(1,0) \begin{pmatrix}
	4 & -2\\
	-2 & 4 \end{pmatrix} \begin{pmatrix}
	\delta_1\\
     \delta_2 \end{pmatrix} = (4, -2) \begin{pmatrix}
     \delta_1\\
     \delta_2 \end{pmatrix} = 4\delta_1 - 2\delta_2 = 0$$
    So, as long as $2\delta_1 = \delta_2$, the condition $\langle d_1, Ad_2 \rangle = 0$ is satisfied
    $$d_2 = \begin{pmatrix}
    \gamma\\
    2\gamma \end{pmatrix}, \;\; \forall \gamma \in \mathbb{R}$$	
	\subsection{Part 2}
	
	Let's calculate the gradient of the function,
	\[f(x) = -12x_2 + 4x_1^2 + 4x_2^2-4x_1x_2, \;\; \nabla f(x) = \begin{pmatrix}
	8x_1 - 4x_2\\
	-12 + 8x_2 - 4x_1 \end{pmatrix} = g(x)\]
	
	Then, we can evaluate $g_0 = \begin{pmatrix}
	-\frac{1}{2} \times 8 - 4 \times -\frac{1}{2}\\
	-12 + 8 + 2
	\end{pmatrix} = \begin{pmatrix}
	-8\\
	-2
	\end{pmatrix}$ by given $x_0 = \begin{pmatrix}
	-\frac{1}{2}\\
	1
	\end{pmatrix}$
	
	In this problem, $d_1$ is given so we don't have to calculate it by $g_0$. So, the next stuff we need is the $\lambda_0 = -\frac{ \langle g_0, d_0 \rangle}{\langle Ad_0, d_0\rangle}$. I would calculate the numerator and enumerator separately.
	
	\[-\langle g_0, d_0 \rangle = -(-8, -2) \begin{pmatrix}
	1\\
	0
	\end{pmatrix} = 8\] 
	\[\langle Ad_0, d_0 \rangle  = (1,0) \begin{pmatrix}
	4 & -2\\
	-2 & 4
	\end{pmatrix} \begin{pmatrix}
	1\\
	0
	\end{pmatrix} = (4, -2) \begin{pmatrix}
	1\\
	0
	\end{pmatrix} = 4\]
	
	For this reason, $\lambda_0 = \frac{8}{4}=2$, and $x^{(1)}$ is, 
	\[x^{(1)} = \begin{pmatrix}
	-1/2\\
	1
	\end{pmatrix} + 2 \begin{pmatrix}
	1\\
	0
	\end{pmatrix} = \begin{pmatrix}
	\frac{3}{2}\\
	1
	\end{pmatrix} \]
	
	In the next iteration, we calculate $x^{(2)}$. To accomplish that, we calculate $g_1 = \begin{pmatrix}
	\frac{3}{2} \times 8 - 4 \times 1\\
	-12 + 8 - 4 \times 1.5
	\end{pmatrix} = \begin{pmatrix}
	8\\
	-10
	\end{pmatrix}$
	
	and by given in the problem, we know $d_1 = \begin{pmatrix}
	1\\
	2
	\end{pmatrix}$, I follow the same routine to calculate the $\lambda_1$
	\[-\langle g_1, d_1 \rangle = -(8, -10) \begin{pmatrix}
	1\\
	2
	\end{pmatrix} = 12\] 
	
	\[\langle Ad_0, d_0 \rangle  = (1,2) \begin{pmatrix}
	4 & -2\\
	-2 & 4
	\end{pmatrix} \begin{pmatrix}
	1\\
	2
	\end{pmatrix} = (0, 6) \begin{pmatrix}
	1\\
	2
	\end{pmatrix} = 12\]
	
	For this reason, $\lambda_1 = 1$ and we can evaluate $x^{(2)}$ as
	\[x^{(2)} = \begin{pmatrix}
	3/2\\
	1
	\end{pmatrix} + 1 \begin{pmatrix}
	1\\
	2
	\end{pmatrix} = \begin{pmatrix}
	\frac{5}{2}\\
	3
	\end{pmatrix} \]
	 
	\subsection{Part 3}
	The visualization has been done in python via matplotlib. Please refer to the source code to see details. Here is the plot. 
		\begin{figure}[htp]
		\centering
		\includegraphics[width=12cm]{problem15_plt1.png}
	\end{figure}

\end{section}


\end{document}